PartialOrderTactic/testing.lean
@@ -2,7 +2,7 @@
 import PartialOrderTactic.Partiarith
 import Lean.Expr
 
-lemma first (a b c: α) [PartialOrder α] (hab : a ≤ b) (hbc : c = b) : a ≤ c := by partiarith
+lemma first (a b c: α) [PartialOrder α] (hab : a ≤ b) (hbc : c = b) : a ≤ c := by partiarith bfs
 
 
 example (a b c d e: α) [PartialOrder α] (hab : a ≤ b) (hac : a ≤ c) (hbc : c = b) (hbd : b ≤ d) (hce : c ≤ e) : a ≤ e := by partiarith
